ECCA_key_lemmas.v
@@ -1,6 +1,7 @@
 Require Export ECCA_typing.
 Require Export ECCA_equiv_lemmas.
 Require Export ECCA_continuations.
+Require Export ECCA_het_comp.
 
 Lemma Cut (g: ECCAenv) (K : cont) (N: ECCAexp) (A B: ECCAexp):
 (ECCA_cont_has_type g K (Cont N A B) ->
@@ -13,7 +14,7 @@ intros. inversion H ; subst ; cbv.
   intros. rewrite <- H1. eapply aT_Let with (n:= N) (m:= M) (A:=A) (B:=(wk B)) (x:=y) (g:=g); assumption.
 Qed.
 
-Lemma weakening (g : ECCAenv) (x : name) (N A A' U : ECCAexp):
+Lemma weakening (g : ECCAenv) (x : name) (N A A' : ECCAexp):
   ECCA_has_type g N A ->
   ECCA_has_type (ctx_cons g x (Assum A')) N A.
 Proof.
@@ -22,6 +23,18 @@ Admitted.
 Lemma def_weakening (g : ECCAenv) (x : name) (N N' A A' : ECCAexp):
   ECCA_has_type g N A ->
   ECCA_has_type (ctx_cons g x (Def N' A')) N A.
+Admitted.
+
+Lemma append_env_weakening (g g': ECCAenv) (N A : ECCAexp):
+  ECCA_has_type g N A ->
+  ECCA_has_type (appendEnv g g') N A.
+Proof.
+Admitted.
+
+Lemma append_env_equiv_weakening (g g': ECCAenv) (e e' : ECCAexp):
+  ECCA_Equiv g e e' ->
+  ECCA_Equiv (appendEnv g g') e e'.
+Proof.
 Admitted.
 
 Lemma equivalence_in_derivation (g: ECCAenv) (N N' M : ECCAexp) (A B : ECCAexp) (x : name):
@@ -47,3 +60,23 @@ intros. inversion H ; subst ; cbv.
   * assumption.
   * apply equivalence_in_derivation with (N := N); assumption.
 Qed. 
+
+Lemma het_compose_equal_fill_hole (K : cont_r) (N: ECCAcomp) :
+  (flattenECCAconf (het_compose_r K (Comp N))) = (fill_hole N (@unrestrict_cont 0 K)).
+Proof.
+  destruct K; simpl; auto.
+Qed.  
+
+Lemma Hetereogeneous_Cut (g g': ECCAenv) (K : cont_r) (M M': ECCAconf) (A B: ECCAexp):
+ECCA_cont_has_type (appendEnv g g') (unrestrict_cont K) (Cont M' A B) ->
+ECCA_has_type g M A ->
+(@ECCA_conf_wf 0 g M) ->
+ECCA_Equiv g M M' ->
+ECCA_has_type (appendEnv g g') (het_compose_r K M) B.
+Proof.
+  intros. induction H1.
+  - erewrite het_compose_equal_fill_hole. apply Cut_modulo_equivalence with (A := A) (N:=M'). assumption. inversion H. assumption. assumption. apply append_env_weakening with (g':=g') in H0. assumption. apply equiv_sym. apply append_env_equiv_weakening with (g':=g') in H2. assumption.
+  - simpl. Admitted.
+
+    
+ 
